combine cfg files

src/CFG/Collecting/CFG_Collect.thy
@@ -1,19 +1,147 @@
 theory CFG_Collect
-  imports CFG_Collect_Edges IMP2_Proc_to_CFG
+  imports "Voblint_IMP2.IMP2_Expr" CFG_Path "Voblint_IMP2.IMP2_Globals" IMP2_Proc_to_CFG
 begin
 
-section \<open>Interprocedural collecting semantics\<close>
+section \<open>CFG collecting semantics\<close>
 
 text \<open>
-  Interprocedural collecting semantics: extends the per-edge transformer
-  with combine triples from combines g:
-    (call, proc_exit, return) contributes
-      { combine_states s t | s in C call, t in C proc_exit }
-    at the return program point.
+  Pointwise CFG collecting semantics over store sets. Normal edges use
+  edge_collect and collect_pp. Interprocedural return flow uses combine triples:
+  (call, proc_exit, return) contributes states built from the call state and
+  the procedure-exit state at the return program point.
 
-  Operational adequacy (pruns_to => cfg_collect) is proved in
-  CFG_Collect_Adeq.
+  Run-to-exit projection is defined in CFG_Collect_Runs.
 \<close>
+
+subsection \<open>Edge transfer\<close>
+
+fun edge_collect :: "edge_action => store set => store set" where
+    "edge_collect EA_Nop           S = S"
+  | "edge_collect (EA_Assign x a)  S = {s(x := aval a s) | s. s : S}"
+  | "edge_collect (EA_Assume b)    S = {s. s \<in> S \<and> bval b s}"
+  | "edge_collect (EA_AssumeNot b) S = {s. s \<in> S \<and> \<not>bval b s}"
+  | "edge_collect EA_Enter           S = enter_state ` S"
+
+lemma edge_collect_empty_set[simp]: "edge_collect a {} = {}"
+  by (cases a) auto
+
+lemma edge_collect_mono:
+  assumes "S \<subseteq> T"
+  shows "edge_collect a S \<subseteq> edge_collect a T"
+  using assms by (cases a) auto
+
+lemma edge_collect_member:
+  "x \<in> edge_collect a S \<longleftrightarrow> (\<exists>s\<in>S. x \<in> edge_collect a {s})"
+  by (cases a) auto
+
+subsection \<open>Path transfer\<close>
+
+text \<open>
+  edges_collect folds edge actions over a path. It ignores the target program
+  point carried with each path step.
+\<close>
+
+fun edges_collect :: "(edge_action * pp) list => store set => store set" where
+  "edges_collect [] S = S"
+| "edges_collect ((a, _) # es) S = edges_collect es (edge_collect a S)"
+
+lemma edges_collect_empty_set[simp]: "edges_collect es {} = {}"
+  by (induction es) auto
+
+lemma edges_collect_mono_strong:
+  "S \<subseteq> T \<Longrightarrow> edges_collect es S \<subseteq> edges_collect es T"
+  apply (induction es S arbitrary: T rule:edges_collect.induct)
+  by (auto simp add: edge_collect_mono)
+
+lemma edges_collect_member:
+  "x \<in> edges_collect es S \<longleftrightarrow> (\<exists>s\<in>S. x \<in> edges_collect es {s})"
+proof (induction es arbitrary: S x)
+  case Nil
+  then show ?case by auto
+next
+  case (Cons e es)
+  obtain a p where ep: "e = (a, p)" by (cases e) auto
+  show ?case unfolding ep
+    by (metis edge_collect_member edges_collect.simps(2) local.Cons)
+qed
+
+lemma edges_collect_memberE[elim]:
+  assumes "x \<in> edges_collect es S"
+  obtains s where "s \<in> S" and "x \<in> edges_collect es {s}"
+  using assms edges_collect_member by blast
+
+lemma edges_collect_append[simp]:
+  "edges_collect (es1 @ es2) S = edges_collect es2 (edges_collect es1 S)"
+  apply (induction es1 arbitrary: S)
+  by auto
+
+lemma edges_collect_nop_append:
+  "edges_collect (es1 @ [(EA_Nop, w)] @ es2) S = edges_collect es2 (edges_collect es1 S)"
+proof (induction es1 arbitrary: S)
+  case Nil
+  show ?case by simp
+next
+  case (Cons e es1)
+  obtain a p where ep: "e = (a, p)" by (cases e) auto
+  show ?case
+    unfolding ep edges_collect.simps edges_collect_append Cons by simp
+qed
+
+lemma mem_edges_collect_from_set:
+  "t \<in> edges_collect es M \<Longrightarrow> \<exists>m\<in>M. t \<in> edges_collect es {m}"
+proof (induction es arbitrary: M t)
+  case Nil
+  then show ?case by simp
+next
+  case (Cons e es)
+  obtain a w where ew: "e = (a, w)" by (cases e) auto
+  obtain M' where M': "M' = edge_collect a M" by simp
+  from Cons.prems ew obtain t': "t \<in> edges_collect es M'"
+    using M' edges_collect.simps(2) by blast
+  from Cons.IH[OF this] obtain m where m: "m \<in> M'" and tm: "t \<in> edges_collect es {m}"
+    by blast
+  from m have "m \<in> edge_collect a M"
+    using M' by auto
+  then obtain m0 where m0: "m0 \<in> M" and mm: "m \<in> edge_collect a {m0}"
+    by (cases a) auto
+  have "t \<in> edges_collect (e # es) {m0}"
+    unfolding ew edges_collect.simps mm tm
+    using mm edges_collect_member tm by blast
+  with m0 show ?case by blast
+qed
+
+lemma edges_collect_offset_path[simp]:
+  "edges_collect (offset_path k es) S = edges_collect es S"
+  by (induction es arbitrary: S) (auto simp: offset_path_def)
+
+subsection \<open>Collecting environments\<close>
+
+text \<open>
+  A collecting environment maps each program point to the set of stores that can
+  appear there during an execution from a fixed initial set.
+\<close>
+
+type_synonym cenv = "pp => store set"
+
+definition collect_pp :: "cfg => cenv => pp => store set" where
+  "collect_pp g \<rho> v =
+     \<Union>{edge_collect a (\<rho> u) | u a. (u, a, v) : edges g}"
+
+lemma collect_pp_mono:
+  "mono (\<lambda>\<rho>. collect_pp g \<rho> v)"
+proof
+  fix rho1 rho2 :: cenv
+  assume "rho1 \<le> rho2"
+  then have "\<forall>u. rho1 u \<subseteq> rho2 u"
+    by (simp add: le_fun_def)
+  then have edge: "\<forall>a u. edge_collect a (rho1 u) \<subseteq> edge_collect a (rho2 u)"
+    using edge_collect_mono by auto
+  then show "collect_pp g rho1 v \<subseteq> collect_pp g rho2 v"
+    unfolding collect_pp_def by auto
+qed
+
+subsection \<open>Interprocedural combine transfer\<close>
+
 
 definition collect_combine_pp :: "cfg \<Rightarrow> cenv \<Rightarrow> pp \<Rightarrow> store set" where
   "collect_combine_pp g \<rho> v =
